ConNF/Counting/Spec.lean
@@ -17,10 +17,56 @@ namespace ConNF
 variable [Params.{u}] [Level] [FOAAssumptions] {β : Λ}
 
 inductive SpecCondition (β : Λ)
-  | atom (A : ExtendedIndex β) (i : κ)
-  | flexible (A : ExtendedIndex β)
+  | atom (A : ExtendedIndex β) (s : Set κ) (t : Set κ)
+  | flexible (A : ExtendedIndex β) (s : Set κ)
   | inflexibleCoe (A : ExtendedIndex β) (h : InflexibleCoePath A)
       (χ : CodingFunction h.δ) (hχ : χ.Strong)
-  | inflexibleBot (A : ExtendedIndex β) (h : InflexibleBotPath A) (i : κ)
+  | inflexibleBot (A : ExtendedIndex β) (h : InflexibleBotPath A) (s : Set κ)
+
+abbrev Spec (β : Λ) := Enumeration (SpecCondition β)
+
+namespace Spec
+
+theorem before_comp_supports (S : Support β) (hS : S.Strong)
+    {i : κ} (hi : i < S.max) {A : ExtendedIndex β}
+    {N : NearLitter} (h : InflexibleCoe A N.1) (hSi : S.f i hi = ⟨A, inr N⟩) :
+    MulAction.Supports (Allowable h.path.δ)
+      ((S.before i hi).comp (h.path.B.cons h.path.hδ)).carrier h.t := by
+  refine (support_supports h.t).mono ?_
+  simp only [Support.comp_carrier, Support.before_carrier, exists_and_left, preimage_setOf_eq]
+  rintro c hc
+  have := Support.Precedes.fuzz A N h c hc
+  rw [h.path.hA] at hSi
+  rw [← hSi] at this
+  obtain ⟨j, hj₁, hj₂, h⟩ := hS.precedes hi _ this
+  exact ⟨j, hj₂, hj₁, h⟩
+
+/-- A specification `σ` specifies an ordered support `S` if each support condition in `S` is
+described in a sensible way by `σ`. -/
+structure Specifies (σ : Spec β) (S : Support β) (hS : S.Strong) : Prop where
+  max_eq_max : S.max = σ.max
+  atom_spec (i : κ) (hi : i < S.max) (A : ExtendedIndex β) (a : Atom) :
+      S.f i hi = ⟨A, inl a⟩ →
+      σ.f i (hi.trans_eq max_eq_max) = SpecCondition.atom A
+        {j | ∃ hj, S.f j hj = ⟨A, inl a⟩} {j | ∃ hj N, S.f j hj = ⟨A, inr N⟩ ∧ a ∈ N}
+  flexible_spec (i : κ) (hi : i < S.max) (A : ExtendedIndex β) (N : NearLitter) :
+      Flexible A N.1 →
+      S.f i hi = ⟨A, inr N⟩ →
+      σ.f i (hi.trans_eq max_eq_max) = SpecCondition.flexible A
+        {j | ∃ hj, ∃ (N' : NearLitter), S.f j hj = ⟨A, inr N⟩ ∧ N'.1 = N'.1}
+  inflexibleCoe_spec (i : κ) (hi : i < S.max) (A : ExtendedIndex β) (N : NearLitter)
+      (h : InflexibleCoe A N.1) (hSi : S.f i hi = ⟨A, inr N⟩) :
+      σ.f i (hi.trans_eq max_eq_max) = SpecCondition.inflexibleCoe A h.path
+        (CodingFunction.code ((S.before i hi).comp (h.path.B.cons h.path.hδ)) h.t
+          (before_comp_supports S hS hi h hSi))
+        (CodingFunction.code_strong _ _ _
+          (Support.comp_strong _ _ (Support.before_strong _ _ _ hS)))
+  inflexibleBot_spec (i : κ) (hi : i < S.max) (A : ExtendedIndex β) (N : NearLitter)
+      (h : InflexibleBot A N.1) :
+      S.f i hi = ⟨A, inr N⟩ →
+      σ.f i (hi.trans_eq max_eq_max) = SpecCondition.inflexibleBot A h.path
+        {j | ∃ hj, S.f j hj = ⟨h.path.B.cons (bot_lt_coe _), inl h.a⟩}
+
+end Spec
 
 end ConNF
